---
title: "STAT 608 HW 7"
author: "Jack Cunningham (jgavc@tamu.edu)"
date: 11/22/2024
date-format: short
format:
  pdf:
    include-in-header:
      - text: |
          \usepackage{amsmath}
editor: visual
engine: knitr
---

1\)

We have the logistic regression model with one predictor:

$$
\log(\frac{\theta(x)}{1-\theta(x)})=\beta_0+\beta_1x
$$

a\)

We apply $e^x$ to both sides:

$$
\frac{\theta(x)}{1-\theta(x)}=e^{\beta_0+\beta_1x}
$$

Multiply both sides by $1-\theta(x)$:

$$
\theta(x)=(1-\theta(x))e^{\beta_0+\beta_1x}
$$

$$
\theta(x)=e^{\beta_0+\beta_1x}-e^{\beta_0+\beta_1x}\theta(x)
$$

$$
\theta(x)+e^{\beta_0+\beta_1x} \theta(x)=e^{\beta_0+\beta_1x}
$$

On left side we factor out $\theta(x)$:

$$
\theta(x)(1+e^{\beta_0+\beta_1x})=e^{\beta_0+\beta_1x}
$$

We are left with the desired result:

$$
\theta(x)=\frac{e^{\beta_0+\beta_1x}}{1+e^{\beta_0+\beta_1x}}
$$

b\)

Starting from our result in a, we multiply by $e^{-(\beta_0+\beta_1x)}/e^{-(\beta_0+\beta_1x)}$:

$$
\theta(x)=(\frac{e^{\beta_0+\beta_1x}}{1+e^{\beta_0+\beta_1x}})\frac{e^{-(\beta_0+\beta_1x)}}{e^{-(\beta_0+\beta_1x)}}
$$

With $e^{-(\beta_0+\beta_1x)}e^{\beta_0+\beta_1x}=1$, we distribute through and are left with the desired result:

$$
\theta(x)=\frac{1}{1+e^{-(\beta_0+\beta_x)}}
$$
